refactored some folders and added some lemmas for GridGraph.v

src/Examples/Topologies/GridGraph.v
@@ -1,32 +1,138 @@
-From StdLib Require Import List Arith Lia.
+From Stdlib Require Import List Bool ZArith.Znat.
+From DatalogRocq Require Import Dataflow.
 Import ListNotations.
-
-Record Graph (Node : Type) := {
-  nodes : Node -> Prop;
-  edge  : Node -> Node -> Prop
-}.
 
 Section GridGraph.
 
-  Variable dims : list nat.
-  Definition Node := Vector.t nat (length dims).
+  Definition Node : Type := list nat.
+  Definition Dimensions : Type := list nat.
 
-  (* All nodes are allowed (infinite grid for now) *)
-  Definition is_node (_ : Node) : Prop := True.
+  Variable dims : Dimensions.
 
+  Fixpoint list_eqb {A : Type} (eqb : A -> A -> bool) (l1 l2 : list A) : bool :=
+    match l1, l2 with
+    | [], [] => true
+    | x :: xs, y :: ys => eqb x y && list_eqb eqb xs ys
+    | _, _ => false
+    end.
+
+  Lemma list_eqb_spec {A : Type}
+      (eqb : A -> A -> bool)
+      (eqb_spec : forall x y : A, BoolSpec (x = y) (x <> y) (eqb x y))
+      (l1 l2 : list A) : BoolSpec (l1 = l2) (l1 <> l2) (list_eqb eqb l1 l2).
+  Proof.
+    revert l2.
+    induction l1 as [|x xs IH]; intros [|y ys]; simpl.
+    - constructor. reflexivity.
+    - constructor. discriminate.
+    - constructor. discriminate.
+    - destruct (eqb_spec x y) as [Hxy | Hxy].
+      + subst y.
+        destruct (IH ys) as [H | H].
+        * subst ys. constructor. reflexivity.
+        * constructor. intros Heq. inversion Heq. contradiction.
+      + constructor. intros Heq. inversion Heq. contradiction.
+  Qed.
+
+  Definition node_eqb (n1 n2 : Node) : bool := list_eqb Nat.eqb n1 n2.
+
+  Lemma node_eqb_spec :
+    forall n1 n2 : Node,
+      BoolSpec (n1 = n2) (n1 <> n2) (node_eqb n1 n2).
+  Proof.
+    unfold node_eqb.
+    apply list_eqb_spec.
+    intros x y. destruct (Nat.eqb_spec x y); constructor; congruence.
+  Qed.
+
+  Definition check_node_in_bounds (n : Node) : bool :=
+    let fix check_dims coords dims :=
+        match coords, dims with
+        | [], [] => true
+        | c :: cs, d :: ds => (c <? d) && check_dims cs ds
+        | _, _ => false
+        end
+    in check_dims n dims.
+
+  Inductive is_graph_node : Dimensions -> Node -> Prop :=
+  | valid_nil : is_graph_node [] []
+  | valid_cons : forall (d : nat) (ds : list nat) (coord : nat) (rest : Node),
+      coord < d ->
+      is_graph_node ds rest ->
+      is_graph_node (d :: ds) (coord :: rest).
+
+  Definition abs (c1 c2 : nat) : nat := Nat.max (c1 - c2) (c2 - c1).
+
+  (* This definition says if a node is n steps away from another node by manhattan distance,
+     and here we don't care about the dimensions *)
+  Inductive manhattan_distance : nat -> Node -> Node -> Prop := 
+  | neighbor_zero_steps : forall n,
+      manhattan_distance 0 n n
+  | neighbor_steps : forall prev_diff next_coord_diff n1 n2 c1 c2,
+      manhattan_distance prev_diff n1 n2 -> 
+      abs c1 c2 = next_coord_diff -> 
+      manhattan_distance (prev_diff + next_coord_diff) (c1 :: n1) (c2 :: n2).
+    
   (* Simple adjacency: differs by +1 on exactly one coordinate *)
-  Definition is_edge (u v : Node) : Prop :=
-    exists i (Hi : i < length dims),
-      Vector.nth v (Fin.of_nat_lt Hi)
-      =
-      S (Vector.nth u (Fin.of_nat_lt Hi)).
+  Inductive is_graph_edge : Dimensions -> Node -> Node -> Prop := 
+  | valid_edge : forall (dims : Dimensions) (u v : Node),
+                 is_graph_node dims u ->
+                 is_graph_node dims v -> 
+                 manhattan_distance 1 u v ->
+                 is_graph_edge dims u v.
 
   (* The actual graph *)
-  Definition GridGraph : Graph Node :=
+  Definition GridGraph : Dataflow.Graph :=
     {|
-      nodes := is_node;
-      edge  := is_edge
+      nodes := is_graph_node dims;
+      edge  := is_graph_edge dims
     |}.
+
+  Theorem good_graph : Dataflow.good_graph GridGraph.
+  Proof.
+    unfold Dataflow.good_graph.
+    intros n1 n2 Hedge.
+    split; inversion Hedge; assumption.
+  Qed.
+
+  Fixpoint all_nodes_h (dims : list nat) : list Node :=
+    match dims with
+    | [] => [[]]
+    | d :: ds =>
+        let rest := all_nodes_h ds in
+        flat_map (fun i => map (fun r => i :: r) rest) (seq 0 d)
+    end.
+  
+  Definition all_nodes : list Node := all_nodes_h dims.
+
+  Theorem all_nodes_h_correct : forall (n : Node),
+    is_graph_node dims n <-> In n (all_nodes_h dims).
+  Proof.
+    intros n. split.
+    - intros Hnode.
+      induction Hnode.
+      + simpl. left. reflexivity.
+      + simpl. 
+        remember (all_nodes_h ds) as rest_nodes. admit.
+    - intros Hin.
+      induction dims.
+      + simpl in Hin. destruct Hin as [Heq | Hnil].
+        * subst. constructor.
+        * inversion Hnil.
+  Admitted.
+
+  Theorem all_nodes_correct : forall (n : Node),
+    is_graph_node dims n <-> In n (all_nodes).
+  Proof.
+    intros n. unfold all_nodes.
+    apply all_nodes_h_correct.
+  Qed.
+
+
+  (* Definition visit_graph_nodes (f : Node -> unit) : unit :=
+  List.iter (fun n => if check_node_in_bounds n then f n else tt) (all_nodes dims).
+ *)
+
 
 End GridGraph.
 
