src/Examples/Layouts/GridLayout.v
@@ -1,0 +1,27 @@
+From Stdlib Require Import List.
+From DatalogRocq Require Import Dataflow GridGraph DependencyGenerator ATLDatalogParams Matmul.
+From Datalog Require Import CompilerExamples.
+From coqutil Require Import Map.Interface Map.Properties Map.Solver.
+Import ListNotations.
+
+Definition three_three_dims : list nat := [3; 3].
+
+Definition three_three_grid_graph := GridGraph three_three_dims.
+
+Definition indexed_layout : list (Node * list nat) := [].
+
+Definition layout (n : Node) : list rule := 
+ match find (fun p => if GridGraph.node_eqb (fst p) n then true else false) indexed_layout with
+  | None => []
+  | Some (_, ris) =>
+      map (fun ri => nth ri datalog_matmul empty_rule) ris
+  end.
+
+Theorem good_layout :
+  Dataflow.good_layout layout three_three_grid_graph.(nodes) datalog_matmul.
+Proof.
+    unfold Dataflow.good_layout.
+    split.
+    - apply Forall_forall. intros. admit.
+    - intros. split.
+Admitted.
